style improvements

theories/base_logic/lib/invariants.v
@@ -6,35 +6,31 @@ From iris.base_logic.lib Require Import wsat.
 Set Default Proof Using "Type".
 Import uPred.
 
-
-Lemma fresh_inv_name (E : gset positive) N : ∃ i, i ∉ E ∧ i ∈ (↑N:coPset).
-Proof.
-  exists (coPpick (↑ N ∖ gset_to_coPset E)).
-  rewrite -elem_of_gset_to_coPset (comm and) -elem_of_difference.
-  apply coPpick_elem_of=> Hfin.
-  eapply nclose_infinite, (difference_finite_inv _ _), Hfin.
-  apply gset_to_coPset_finite.
-Qed.
+(** Semantic Invariants *)
+Definition inv_def `{!invG Σ} (N : namespace) (P : iProp Σ) : iProp Σ :=
+  (□ ∀ E, ⌜↑N ⊆ E⌝ → |={E,E ∖ ↑N}=> ▷ P ∗ (▷ P ={E ∖ ↑N,E}=∗ True))%I.
+Definition inv_aux : seal (@inv_def). by eexists. Qed.
+Definition inv {Σ i} := inv_aux.(unseal) Σ i.
+Definition inv_eq : @inv = @inv_def := inv_aux.(seal_eq).
+Instance: Params (@inv) 3 := {}.
+Typeclasses Opaque inv.
 
 (** * Invariants *)
 Section inv.
   Context `{!invG Σ}.
+  Implicit Types i : positive.
+  Implicit Types N : namespace.
+  Implicit Types E : coPset.
+  Implicit Types P Q R : iProp Σ.
 
-  (** Internal backing store of invariants *)
-  Definition internal_inv_def (N : namespace) (P : iProp Σ) : iProp Σ :=
+  (** ** Internal model of invariants *)
+  Definition own_inv (N : namespace) (P : iProp Σ) : iProp Σ :=
     (∃ i P', ⌜i ∈ (↑N:coPset)⌝ ∧ ▷ □ (P' ↔ P) ∧ ownI i P')%I.
-  Definition internal_inv_aux : seal (@internal_inv_def). by eexists. Qed.
-  Definition internal_inv := internal_inv_aux.(unseal).
-  Definition internal_inv_eq : @internal_inv = @internal_inv_def := internal_inv_aux.(seal_eq).
-  Typeclasses Opaque internal_inv.
 
-  Global Instance internal_inv_persistent N P : Persistent (internal_inv N P).
-  Proof. rewrite internal_inv_eq /internal_inv; apply _. Qed.
-
-  Lemma internal_inv_open E N P :
-  ↑N ⊆ E → internal_inv N P ={E,E∖↑N}=∗ ▷ P ∗ (▷ P ={E∖↑N,E}=∗ True).
+  Lemma own_inv_open E N P :
+    ↑N ⊆ E → own_inv N P ={E,E∖↑N}=∗ ▷ P ∗ (▷ P ={E∖↑N,E}=∗ True).
   Proof.
-    rewrite internal_inv_eq /internal_inv_def uPred_fupd_eq /uPred_fupd_def.
+    rewrite uPred_fupd_eq /uPred_fupd_def.
     iDestruct 1 as (i P') "(Hi & #HP' & #HiP)".
     iDestruct "Hi" as % ?%elem_of_subseteq_singleton.
     rewrite {1 4}(union_difference_L (↑ N) E) // ownE_op; last set_solver.
@@ -46,18 +42,27 @@ Section inv.
     iApply "HP'". iFrame.
   Qed.
 
-  Lemma internal_inv_alloc N E P : ▷ P ={E}=∗ internal_inv N P.
+  Lemma fresh_inv_name (E : gset positive) N : ∃ i, i ∉ E ∧ i ∈ (↑N:coPset).
   Proof.
-    rewrite internal_inv_eq /internal_inv_def uPred_fupd_eq. iIntros "HP [Hw $]".
+    exists (coPpick (↑ N ∖ gset_to_coPset E)).
+    rewrite -elem_of_gset_to_coPset (comm and) -elem_of_difference.
+    apply coPpick_elem_of=> Hfin.
+    eapply nclose_infinite, (difference_finite_inv _ _), Hfin.
+    apply gset_to_coPset_finite.
+  Qed.
+
+  Lemma own_inv_alloc N E P : ▷ P ={E}=∗ own_inv N P.
+  Proof.
+    rewrite uPred_fupd_eq. iIntros "HP [Hw $]".
     iMod (ownI_alloc (.∈ (↑N : coPset)) P with "[$HP $Hw]")
       as (i ?) "[$ ?]"; auto using fresh_inv_name.
     do 2 iModIntro. iExists i, P. rewrite -(iff_refl True%I). auto.
   Qed.
 
-  Lemma internal_inv_alloc_open N E P :
-    ↑N ⊆ E → (|={E, E∖↑N}=> internal_inv N P ∗ (▷P ={E∖↑N, E}=∗ True))%I.
+  Lemma own_inv_alloc_open N E P :
+    ↑N ⊆ E → (|={E, E∖↑N}=> own_inv N P ∗ (▷P ={E∖↑N, E}=∗ True))%I.
   Proof.
-    rewrite internal_inv_eq /internal_inv_def uPred_fupd_eq. iIntros (Sub) "[Hw HE]".
+    rewrite uPred_fupd_eq. iIntros (Sub) "[Hw HE]".
     iMod (ownI_alloc_open (.∈ (↑N : coPset)) P with "Hw")
       as (i ?) "(Hw & #Hi & HD)"; auto using fresh_inv_name.
     iAssert (ownE {[i]} ∗ ownE (↑ N ∖ {[i]}) ∗ ownE (E ∖ ↑ N))%I
@@ -75,85 +80,62 @@ Section inv.
     rewrite assoc_L -!union_difference_L //; set_solver.
   Qed.
 
-  (** Invariants API *)
-  Definition inv_def (N: namespace) (P: iProp Σ) : iProp Σ :=
-    (□ (∀ E, ⌜↑N ⊆ E⌝ → |={E,E ∖ ↑N}=> ▷ P ∗ (▷ P ={E ∖ ↑N,E}=∗ True)))%I.
-  Definition inv_aux : seal (@inv_def). by eexists. Qed.
-  Definition inv := inv_aux.(unseal).
-  Definition inv_eq : @inv = @inv_def := inv_aux.(seal_eq).
-  Typeclasses Opaque inv.
+  Lemma own_inv_to_inv M P: own_inv M P  -∗ inv M P.
+  Proof.
+    iIntros "#I". rewrite inv_eq. iIntros (E H).
+    iPoseProof (own_inv_open with "I") as "H"; eauto.
+  Qed.
 
-  (** Properties about invariants *)
-  Global Instance inv_contractive N: Contractive (inv N).
+  (** ** Public API of invariants *)
+  Global Instance inv_contractive N : Contractive (inv N).
   Proof. rewrite inv_eq. solve_contractive. Qed.
 
   Global Instance inv_ne N : NonExpansive (inv N).
   Proof. apply contractive_ne, _. Qed.
 
-  Global Instance inv_proper N: Proper (equiv ==> equiv) (inv N).
+  Global Instance inv_proper N : Proper (equiv ==> equiv) (inv N).
   Proof. apply ne_proper, _. Qed.
 
-  Global Instance inv_persistent M P: Persistent (inv M P).
-  Proof. rewrite inv_eq. typeclasses eauto. Qed.
+  Global Instance inv_persistent N P : Persistent (inv N P).
+  Proof. rewrite inv_eq. apply _. Qed.
 
   Lemma inv_acc N P Q:
     inv N P -∗ ▷ □ (P -∗ Q ∗ (Q -∗ P)) -∗ inv N Q.
   Proof.
-    iIntros "#I #Acc". rewrite inv_eq.
-    iModIntro. iIntros (E H). iDestruct ("I" $! E H) as "#I'".
-    iApply fupd_wand_r. iFrame "I'".
-    iIntros "(P & Hclose)". iSpecialize ("Acc" with "P").
-    iDestruct "Acc" as "[Q CB]". iFrame.
-    iIntros "Q". iApply "Hclose". now iApply "CB".
+    rewrite inv_eq. iIntros "#HI #Acc !>" (E H).
+    iMod ("HI" $! E H) as "[HP Hclose]".
+    iDestruct ("Acc" with "HP") as "[$ HQP]".
+    iIntros "!> HQ". iApply "Hclose". iApply "HQP". done.
   Qed.
 
   Lemma inv_iff N P Q : ▷ □ (P ↔ Q) -∗ inv N P -∗ inv N Q.
   Proof.
-    iIntros "#HPQ #I". iApply (inv_acc with "I").
-    iNext. iIntros "!# P". iSplitL "P".
+    iIntros "#HPQ #HI". iApply (inv_acc with "HI").
+    iIntros "!> !# HP". iSplitL "HP".
     - by iApply "HPQ".
-    - iIntros "Q". by iApply "HPQ".
-  Qed.
-
-  Lemma inv_to_inv M P: internal_inv M P  -∗ inv M P.
-  Proof.
-    iIntros "#I". rewrite inv_eq. iIntros (E H).
-    iPoseProof (internal_inv_open with "I") as "H"; eauto.
+    - iIntros "HQ". by iApply "HPQ".
   Qed.
 
   Lemma inv_alloc N E P : ▷ P ={E}=∗ inv N P.
   Proof.
-    iIntros "P". iPoseProof (internal_inv_alloc  N E with "P") as "I".
-    iApply fupd_mono; last eauto.
-    iApply inv_to_inv.
+    iIntros "HP". iApply own_inv_to_inv.
+    iApply (own_inv_alloc N E with "HP").
   Qed.
 
   Lemma inv_alloc_open N E P :
     ↑N ⊆ E → (|={E, E∖↑N}=> inv N P ∗ (▷P ={E∖↑N, E}=∗ True))%I.
   Proof.
-    iIntros (H). iPoseProof (internal_inv_alloc_open _ _ _ H) as "H".
-    iApply fupd_mono; last eauto.
-    iIntros "[I H]"; iFrame; by iApply inv_to_inv.
+    iIntros (?). iMod own_inv_alloc_open as "[HI $]"; first done.
+    iApply own_inv_to_inv. done.
   Qed.
 
   Lemma inv_open E N P :
     ↑N ⊆ E → inv N P ={E,E∖↑N}=∗ ▷ P ∗ (▷ P ={E∖↑N,E}=∗ True).
   Proof.
-    rewrite inv_eq /inv_def; iIntros (H) "#I". by iApply "I".
+    rewrite inv_eq /inv_def; iIntros (?) "#HI". by iApply "HI".
   Qed.
 
-  Lemma inv_open_strong E N P :
-    ↑N ⊆ E → inv N P ={E,E∖↑N}=∗ ▷ P ∗ ∀ E', ▷ P ={E',↑N ∪ E'}=∗ True.
-  Proof.
-      iIntros (?) "Hinv".      iPoseProof (inv_open (↑ N) N P with "Hinv") as "H"; first done.
-      rewrite difference_diag_L.
-      iPoseProof (fupd_mask_frame_r _ _ (E ∖ ↑ N) with "H") as "H"; first set_solver.
-      rewrite left_id_L -union_difference_L //. iMod "H" as "[$ H]"; iModIntro.
-      iIntros (E') "HP".
-      iPoseProof (fupd_mask_frame_r _ _ E' with "(H HP)") as "H"; first set_solver.
-        by rewrite left_id_L.
-  Qed.
-
+  (** ** Proof mode integration *)
   Global Instance into_inv_inv N P : IntoInv (inv N P) N := {}.
 
   Global Instance into_acc_inv N P E:
@@ -165,6 +147,20 @@ Section inv.
     iIntros (?) "#Hinv _". iApply "Hinv"; done.
   Qed.
 
+  (** ** Derived properties *)
+  Lemma inv_open_strong E N P :
+    ↑N ⊆ E → inv N P ={E,E∖↑N}=∗ ▷ P ∗ ∀ E', ▷ P ={E',↑N ∪ E'}=∗ True.
+  Proof.
+    iIntros (?) "Hinv".
+    iPoseProof (inv_open (↑ N) N P with "Hinv") as "H"; first done.
+    rewrite difference_diag_L.
+    iPoseProof (fupd_mask_frame_r _ _ (E ∖ ↑ N) with "H") as "H"; first set_solver.
+    rewrite left_id_L -union_difference_L //. iMod "H" as "[$ H]"; iModIntro.
+    iIntros (E') "HP".
+    iPoseProof (fupd_mask_frame_r _ _ E' with "(H HP)") as "H"; first set_solver.
+    by rewrite left_id_L.
+  Qed.
+
   Lemma inv_open_timeless E N P `{!Timeless P} :
     ↑N ⊆ E → inv N P ={E,E∖↑N}=∗ P ∗ (P ={E∖↑N,E}=∗ True).
   Proof.
@@ -172,23 +168,22 @@ Section inv.
     iIntros "!> {$HP} HP". iApply "Hclose"; auto.
   Qed.
 
-  (* Weakening of semantic invariants *)
-  Lemma inv_proj_l N P Q: inv N (P ∗ Q) -∗ inv N P.
+  Lemma inv_sep_l N P Q : inv N (P ∗ Q) -∗ inv N P.
   Proof.
-    iIntros "#I". iApply inv_acc; eauto.
-    iNext. iIntros "!# [$ Q] P"; iFrame.
+    iIntros "#HI". iApply inv_acc; eauto.
+    iIntros "!> !# [$ $] $".
   Qed.
 
-  Lemma inv_proj_r N P Q: inv N (P ∗ Q) -∗ inv N Q.
+  Lemma inv_sep_r N P Q : inv N (P ∗ Q) -∗ inv N Q.
   Proof.
-    rewrite (bi.sep_comm P Q). eapply inv_proj_l.
+    rewrite (comm _ P Q). eapply inv_sep_l.
   Qed.
 
-  Lemma inv_split N P Q: inv N (P ∗ Q) -∗ inv N P ∗ inv N Q.
+  Lemma inv_sep N P Q : inv N (P ∗ Q) -∗ inv N P ∗ inv N Q.
   Proof.
     iIntros "#H".
-    iPoseProof (inv_proj_l with "H") as "$".
-    iPoseProof (inv_proj_r with "H") as "$".
+    iPoseProof (inv_sep_l with "H") as "$".
+    iPoseProof (inv_sep_r with "H") as "$".
   Qed.
 
 End inv.
